\begin{exercise}{20}
 Consider the following grammar $G$:
 \begin{align*}
    S ~\to~ & Scc \mid Ac \\
    A ~\to~ & Aab \mid a \mid aBb \\
    B ~\to~ & dA
 \end{align*}
 \begin{enumerate}[(a)]
    \item Show that $G \notin LL(1)$.
    \item Transform $G$ into an equivalent grammar in $LL(1)$, i.e. provide a grammar $G' \in LL(1)$ such that $L(G') = L(G)$.
    \item Prove that $G'$ has the $LL(1)$ property.
 \end{enumerate}

\end{exercise}

\begin{solution}
\begin{enumerate}[(a)]
\item It is $a \in \la(A \to a)$ and $a \in \la(A \to aBb)$.
Therefore $\la(A \to a) \cap \la(A \to aBb) \neq \emptyset$ and $G \not\in LL(1)$.

\item We eliminate the left recursion for all nonterminals.

We start with $S$:
\begin{align*}
    S  ~\to~ & AcS' \\
    S' ~\to~ & ccS' \mid \varepsilon \\
    A  ~\to~ & Aab \mid a \mid aBb \\
    B  ~\to~ & dA
\end{align*}
Next we remove the left recursion for $A$:
\begin{align*}
    S  ~\to~ & AcS' \\
    S' ~\to~ & ccS' \mid \varepsilon \\
    A  ~\to~ & aA' \mid aBbA' \\
    A' ~\to~ & abA' \mid \varepsilon \\
    B  ~\to~ & dA
\end{align*}
Finally, we apply left-factorization for the rules of $A$:
\begin{align*}
    S  ~\to~ & AcS' \\
    S' ~\to~ & ccS' \mid \varepsilon \\
    A  ~\to~ & aC \\
    C  ~\to~ & A' \mid BbA' \\
    A' ~\to~ & abA' \mid \varepsilon \\
    B  ~\to~ & dA
\end{align*}
The resulting grammar is the grammar $G'$.

\item We prove that $G' \in LL(1)$ by computing the lookahead sets.
\begin{center}
\begin{tabular}[h]{c|c}
    Rule & $\la$ \\
    \hline \hline
    $S  ~\to~ AcS' $ & $\set{a}$ \\
    \hline
    $S' ~\to~ ccS' $ & $\set{c}$ \\
    $S' ~\to~ \varepsilon $ & $\set{\varepsilon}$ \\
    \hline
    $A  ~\to~ aC $ & $\set{a}$ \\
    \hline
    $C  ~\to~ A' $ & $\set{a,b,c}$ \\
    $C  ~\to~ BbA' $ & $\set{d}$ \\
    \hline
    $A' ~\to~ abA' $ & $\set{a}$ \\
    $A' ~\to~ \varepsilon $ & $\set{b,c}$ \\
    \hline
    $B  ~\to~ dA$ & $\set{d}$
\end{tabular}
\end{center}
For every nonterminal it holds that the intersection of their lookahead sets is empty.
Therefore $G' \in LL(1)$.

\end{enumerate}
\end{solution}

